** Assignment 6
#+TITLE: Math 115 A1
#+LaTeX_CLASS: article
#+LaTeX_CLASS_OPTIONS: [article,letterpaper,times,10pt,margin=0.5in]
#+LATEX_HEADER: \usepackage[margin=0.3in]{geometry}
1. Partial fraction decomposition:
   $\frac{x^2-2x-1}{(x-1)^2(x^2+1)}=\frac{Ax+C}{(x-1)^2}+\frac{Bx+D}{x^2+1}$,
   with constants determined by the system
   | x^3 | x^2 | x^1 | x^0 |
   |-----+-----+-----+-----|
   | A   | C   | A   | C   |
   | B   | D   | -2D | D   |
   |     | -2B | B   |     |
   |-----+-----+-----+-----|
   | 0   | 1   | -2  | -1  |
   So that $A=-B=1, C=-2 D=1$, and \\
   $\int\frac{x^2-2x-1}{(x-1)^2(x^2+1)}\,dx = \int \frac{x-2}{(x-1)^2} -\frac{x-1}{x^2+1} \,dx
    = \int (x-1)^{-1}-(x-1)^{-2}\,dx - \int \frac{(x^2+1)'/2}{x^2+1}\,dx + \int \frac{dx}{1+x^2}
    = \ln \frac{|x-1|}{\sqrt{x^2+1}} + \frac{1}{x-1} + \arctan x + C$.
2. Partial fraction decomposition:
    $\frac{1}{(1+x)(1-x+x^2)} = \frac{B}{1+x} + \frac{Cx+D}{1-x+x^2}$,
    where the constants are determined from
   | x^2 | x^1 | x^0 |
   |-----+-----+-----|
   | B   | -B  | D   |
   | C   | C   |     |
   |     | D   |     |
   |-----+-----+-----|
   | 0   | 0   | 1   |
   Hence $B=-C=\frac{1}{3}, D=\frac{2}{3}$, and \\
   $\int 1-\frac{1}{1+x^3}\,dx
      = x + \frac{1}{3} \left(\int\frac{x-2}{1-x+x^2}-\frac{1}{1+x}\,dx\right)
      = x - \frac{\ln|1+x|}{3} + \frac{1}{3}\int\frac{x-\frac{1}{2}+\frac{3}{2}}{(x-\frac{1}{2})^2-\left(\frac{\sqrt3}{2}\right)^2}\,dx
      = x - \frac{\ln|1+x|}{3} + \frac{\ln|x^2-x+1|}{6} - \frac{1}{\sqrt3}\arctan(\frac{2x-1}{\sqrt3})+C$.
3. $I=\int\frac{dx}{\sqrt[3]{x}+\sqrt[4]{x}}
      = 12\int\frac{u^{11}}{u^4+u^3}du$, where $u:=\sqrt[12]x,12u^{11}\,du=dx$, and\\
   $\frac{I}{12} = \int\frac{u^8}{1+u}du
      = \int\frac{(v-1)^8}{v}dv
      = \int v^7-8v^6 + {{8}\choose{2}} v^5- {{8}\choose{3}} v^4
        {} + 70v^3 - 56v^2 + 28u - 8\, dx
        {} + \ln (1+\sqrt[12]{x}) \\
      = \frac{(1+u)^8}{8} - 8\frac{(1+u)^7}{7} + 28\frac{(1+u)^6}{6}
        {} - 56\frac{(1+u)^5}{5} + 70\frac{(1+u)^4}{4} - 56\frac{(1+u)^3}{3}
        {} + 28\frac{(1+u)^2}{2} - 8(1+u) + \ln(1+\sqrt[12]{x}) + C \\
      = -\sqrt[12]{x} + \frac{1}{2}x^{1/6} - \frac{1}{3}x^{1/4}
        {} + \frac{1}{4} x^{1/3} -\frac{1}{5}x^{5/12} + \frac{1}{6}x^{1/2}
        {} -\frac{1}{7}x^{7/12} + \frac{1}{8}x^{2/3} + \ln (1+\sqrt[12]{x}) + C$.
4. $I=\int\frac{\sqrt{1+\ln x}}{x\ln x}dx = \int\frac{\sqrt u\,du}{u-1}$, where $u=1+\ln x, xu'=1, v: = \sqrt{u}, 2v'u=1$.\\
    $I = 2(v+\int\frac{dv}{v^2-1}) = 2(\sqrt{1+\ln x} - \tanh^{-1}(\sqrt{1+\ln x}) + C
       = 2\sqrt{1+\ln x} + \ln\left(\frac{1-\sqrt{1+\ln x}}{1+\sqrt{1+\ln x}}\right) + C$,
    using result of question 3 from Assignment 3.
5. $\int_0^1 x^2\ln(1+x)\,dx = \int_{u:=x+1=1}^2(u-1)^2\ln u\,du
       = \int_1^2 u^2\ln u - 2u\ln u+1\ln u\,du \\
       = \left[\frac{u^3}{3}\ln u-\int \frac{u^3}{3}\frac{1}{u}\,du\right]_1^2
         {} - 2\left[\frac{u^2}{2}\ln u-\frac{u^2}{4}\right]_1^2
         {} + \left[u\ln u - x\right]_1^2
        = \frac{2\ln 2}{3}-\frac{5}{18}$.
6. $\int\frac{dx}{1+\cos x}=\int\frac{dx}{2\cos^2(x/2)}=\tan\frac{x}{2}+C$.
7. $\int_1^9\frac{dx}{\sqrt[3]{x-9}}=\lim_{x\to9}\int_1^x(t-9)^{-1/3}\,d(t-9)
       = \lim_{x\to0^-}\frac{3}{2}(x^{2/3}-(-8)^{2/3})
       = -6$, where we only consider the real (third) roots.
8. $I=\int_0^1\frac{\ln x}{\sqrt{x}}\,dx=\int_0^1 2\frac{\ln u}{u}\,2udu$ where $u=\sqrt x, 2u'u=1$.
   Hence $I=4(-1-\lim_{x\to0^+}(x\ln x-x))$. \\
   Now $\lim_{x\to0^+}\frac{\ln x}{1/x}=\lim_{x\to0^+}\frac{1/x}{-1/x^2}=0$. Thus $I=-4$.
9. $\int_0^\infty\frac{e^x}{e^{2x}+3}\,dx=\int_{u:=e^x=1}^\infty\frac{du}{u^2+3}
       = \frac{\sqrt{3}}{3}(\lim_{y\to\infty}\arctan\frac{y}{\sqrt3}-\frac{\pi}{6})
       = \frac{\pi}{3\sqrt3}$.
10. $\int_{-\infty}^\infty e^{-|x|}\,dx=2\int_0^\infty e^{-x}=2$.
11. $\int_1^\infty0\,dx\leq\int_1^\infty\frac{x}{\sqrt{1+x^6}}\,dx\leq\int_1^\infty\frac{x}{\sqrt x^6}\,dx
       = \int_1^\infty x^{-2}=1$.
12. $\int_1^\infty0\,dx\leq\int_0^\infty\frac{\arctan x}{2+e^x}\,dx\leq\frac{\pi}{2}\int_0^\infty\frac{dx}{2+e^x}
       \leq \frac{\pi}{2}\int_0^\infty e^{-x}\,dx = \frac{\pi}{2}$.
